Capless/Subst/Term/Subtyping.lean
@@ -158,4 +158,14 @@ theorem ESubtyp.subst
     apply ESubtyp.type
     apply hs.subst; trivial
 
+theorem ESubtyp.narrow
+  (h : ESubtyp (Γ.var T) E1 E2)
+  (hs : CSubtyp Γ T' T) :
+  ESubtyp (Γ.var T') E1 E2 := by
+  rw [<- EType.rename_id (E := E1), <- EType.rename_id (E := E2)]
+  apply ESubtyp.subst
+  { trivial }
+  { apply VarSubst.narrow
+    trivial }
+
 end Capless
